model

SmartContracts/ModellingOfBugs/DeusFinacePriceOracleManipulation/lending copy.dfy
@@ -25,14 +25,17 @@ type Address = Account
 
 class LendingContract  {
 
-  var collateral : nat;
+  var collateral : real;
+  var token1 : real;
+  var token2 : real;
+  ghost var inv : real;
   // var reservetime : real;
   // var lastprice1 : nat;
   // var lastprice2 : nat;
   // var positive : bool;
 
-  function method customized_price (data1 : nat, data2 : nat) : nat
-    requires data2 != 0
+  function method customized_price (data1 : real, data2 : real) : real
+    requires data2 != 0.0
   {
     data1 / data2
   }
@@ -45,38 +48,92 @@ class LendingContract  {
   //   (((lastprice1 as real - data1 as real)  * reservetime + lastprice1 as real)/((lastprice2 as real - data2 as real)  * reservetime + lastprice2 as real)).Floor as nat
   // }
 
-  method getdata1() returns (data1 : nat)
-    ensures data1 != 0
-  {data1 := havoc();}
+  predicate valid()
+    reads this
+  {
+    token1 * token2 == inv
+  }
 
-  method getdata2() returns (data2 : nat)
-    ensures data2 != 0
-  {data2 := havoc();}
+  method mutate () returns (data1m : real, data2m : real)
+    requires valid()
+    requires token2 != 0.0
+
+    // reads this
+    modifies this
+
+    ensures data2m != 0.0
+    ensures valid()
+  {
+    var m : real := mut();
+    data1m := token1 * m;
+    data2m := token2 / m;
+    calc
+    {
+      inv;
+      token1 * token2;
+      token1 * m * token2 / m;
+      (token1 * m) * (token2 / m);
+      data1m * data2m;
+      inv;
+    }
+    update(data1m, data2m);
+  }
+
+  method update (tok1 : real, tok2 : real)
+    requires valid()
+    requires tok1 * tok2 == inv
+    requires tok2 != 0.0
+
+    modifies this
+
+    ensures valid()
+    ensures token2 != 0.0
+  {
+    token1 := tok1;
+    token2 := tok2;
+  }
 
   // predicate mutate(data1: nat, data2 : nat, r1: Try<()>, amount :nat)
   // {
   //   transactions(amount, data1 * mutation(), data2 / mutation()) == r1
   // }
 
-  method transactions(amount : nat, data1 : nat, data2 : nat) returns (r1: Try<()>, price : nat)
-    requires data2 != 0
+  method transactions(amount : real, data1 : real, data2 : real) returns (r1: Try<()>, price : real, mutationPrice : real)
+    requires data2 != 0.0
+    requires valid()
 
     modifies this
 
-    ensures  r1.Revert? ==> forall m : nat :: 0 < m < 10 ==> customized_price(data1* m,(if data2/m == 0 then 1 else data2/m)) * collateral < amount
+    ensures  r1.Revert? ==>  mutationPrice * collateral < amount
+    // ensures price ==
 
   {
+    assume(data1 * data2 == inv);
+    update(data1, data2);
     collateral := havoc();
     price := customized_price(data1,data2);
     if (price * collateral < amount)
     {
       r1 := Revert();
-
+      var mdata1 : real, mdata2 : real;
+      assert(token2 != 0.0);
+      mdata1, mdata2 := mutate();
+      mutationPrice := customized_price(mdata1,mdata2);
     }
     else
-    {r1 := Success(());}
+    {
+      r1 := Success(());
+      mutationPrice := 0.0;
+    }
   }
+
+  // lemma mutation(data1 : real, data2: real)
+  //   requires m != 0.0
+  //   ensures data1 * data2 == (data1 * m) * (data2 / m)
 }
 
-method {:extern} havoc() returns (a: nat)
-  ensures a != 0
+method {:extern} havoc() returns (a: real)
+  ensures a != 0.0
+
+method {:extern} mut() returns (a: real)
+  ensures 0.0 < a < 10.0
